LinearAssemblyLanguage.thy
@@ -1,0 +1,32 @@
+theory LinearAssemblyLanguage
+imports FiniteMap BasicComputation
+begin
+
+datatype assembly =
+  AAssm int
+| CAssm "register set" computation
+| JAssm "comparison set" code_label
+
+type_synonym linear_assembly_program = "code_label \<leadsto> assembly list"
+
+type_synonym assembly_state = "memory \<times> int option \<times> int \<times> assembly list" (* \<mu>, a, d, pc *)
+
+fun eval_linear_assembly :: "linear_assembly_program \<Rightarrow> assembly_state \<Rightarrow> assembly_state option" where
+  "eval_linear_assembly \<Pi> (\<mu>, a, d, []) = None"
+| "eval_linear_assembly \<Pi> (\<mu>, a, d, AAssm x # \<pi>) = Some (\<mu>, Some x, d, \<pi>)"
+| "eval_linear_assembly \<Pi> (\<mu>, Some a, d, CAssm dst cmp # \<pi>) = (
+    let n = compute cmp (\<mu> a) a d
+    in Some (
+      if M \<in> dst then \<mu>(a := n) else \<mu>, 
+      Some (if A \<in> dst then n else a), 
+      if D \<in> dst then n else d, 
+      \<pi>))"
+| "eval_linear_assembly \<Pi> (\<mu>, None, d, CAssm dst cmp # \<pi>) = None"
+| "eval_linear_assembly \<Pi> (\<mu>, a, d, JAssm jmp s # \<pi>) = (
+    if should_jump d jmp
+    then case lookup \<Pi> s of 
+        Some \<pi>' \<Rightarrow> Some (\<mu>, None, d, \<pi>')
+      | None \<Rightarrow> None
+    else Some (\<mu>, None, d, \<pi>))"
+
+end
